WIP wp_rule hash + fix hash spec

theories/rules/rules_Hash.v
@@ -3,7 +3,7 @@ From iris.program_logic Require Export weakestpre ectx_lifting.
 From iris.proofmode Require Import proofmode.
 From iris.algebra Require Import frac.
 From cap_machine Require Import machine_base.
-From cap_machine Require Export rules_base region.
+From cap_machine Require Export rules_base region logical_mapsto.
 
 Section cap_lang_rules.
   Context `{ceriseg: ceriseG Σ}.
@@ -22,15 +22,15 @@ Section cap_lang_rules.
   Definition reg_allows_hash (lregs : LReg) (r : RegName) p b e a v :=
     lregs !! r = Some (LCap p b e a v) ∧ readAllowed p = true.
 
-  Definition hash_lmemory_region (lm : LMem) (b e : Addr) (v : Version) :=
-    let instructions : list LWord :=
-      map snd
-        ((map_to_list
-            (filter (fun mem_addr => (laddr_get_addr (fst mem_addr)) ∈ (finz.seq_between b e)
-                                  /\ (laddr_get_version (fst mem_addr)) = v)
-               lm)))
-    in
-    hash (fmap lword_get_word instructions).
+  (* Definition hash_lmemory_region (lm : LMem) (b e : Addr) (v : Version) := *)
+  (*   let instructions : list LWord := *)
+  (*     map snd *)
+  (*       ((map_to_list *)
+  (*           (filter (fun mem_addr => (laddr_get_addr (fst mem_addr)) ∈ (finz.seq_between b e) *)
+  (*                                 /\ (laddr_get_version (fst mem_addr)) = v) *)
+  (*              lm))) *)
+  (*   in *)
+  (*   hash (fmap lword_get_word instructions). *)
 
   Inductive Hash_failure (lregs: LReg) (dst src: RegName) (lmem : LMem) :=
   | Hash_fail_const lw:
@@ -56,8 +56,9 @@ Section cap_lang_rules.
       incrementLPC (<[ dst := LInt (hash_lmemory_region lmem b e v)]> lregs) = Some lregs' ->
       Hash_spec lregs dst src lmem lregs' NextIV
   | Hash_spec_failure:
-      Hash_failure lregs dst src lmem ->
-      Hash_spec lregs dst src lmem lregs' FailedV.
+    lregs = lregs' ->
+    Hash_failure lregs dst src lmem ->
+    Hash_spec lregs dst src lmem lregs' FailedV.
 
   Definition allow_hash_map_or_true r (lregs : LReg) (lmem : LMem):=
     ∃ p b e a v, read_reg_inr lregs r p b e a v ∧
@@ -81,75 +82,67 @@ Section cap_lang_rules.
     - contradiction Hrega. done.
   Qed.
 
-  (* Lemma mem_eq_implies_allow_hash_map: *)
-  (*   ∀ (lregs : LReg) (lmem : LMem) (src : RegName) (lw : LWord) p b e a v, *)
-  (*     lmem = <[(a, v):=lw]> ∅ *)
-  (*     → lregs !! src = Some (LCap p b e a v) *)
-  (*     → allow_hash_map_or_true src lregs lmem. *)
-  (* Proof. *)
-  (*   intros lregs lmem src lw p b e a v Hmem Hrsrc. *)
-  (*   exists p,b,e,a,v; split. *)
-  (*   - unfold read_reg_inr. by rewrite Hrsrc. *)
-  (*   - case_decide; last done. *)
-  (*     exists lw. simplify_map_eq. auto. *)
-  (* Qed. *)
+  Lemma incrementLPC_incrementPC_some regs regs' :
+    incrementLPC regs = Some regs' ->
+    incrementPC (lreg_strip regs) = Some (lreg_strip regs').
+  Proof.
+    rewrite /incrementPC /incrementLPC.
+    intros Hlpc.
+    rewrite /lreg_strip lookup_fmap; cbn.
+    destruct (regs !! PC) as [lw|] eqn:Heq ; rewrite Heq; cbn in *; last done.
+    destruct_lword lw; cbn in *; try done.
+    destruct (a + 1)%a; last done.
+    simplify_eq.
+    by rewrite fmap_insert.
+  Qed.
 
-  (* Lemma mem_neq_implies_allow_load_map: *)
-  (*   ∀ (lregs : LReg) (lmem : LMem) (r2 : RegName) (pc_a : Addr) (pca_v : Version) *)
-  (*     (lw lw' : LWord) p b e a v, *)
-  (*     (a ≠ pc_a \/ v <> pca_v) *)
-  (*     → lmem = <[(pc_a, pca_v):= lw]> (<[(a, v) := lw']> ∅) *)
-  (*     → lregs !! r2 = Some (LCap p b e a v) *)
-  (*     → allow_load_map_or_true r2 lregs lmem. *)
-  (* Proof. *)
-  (*   intros lregs lmem r2 pc_a pca_v lw lw' p b e a v H4 Hrr2 Hreg2. *)
-  (*   exists p,b,e,a,v; split. *)
-  (*   - unfold read_reg_inr. by rewrite Hreg2. *)
-  (*   - case_decide; last done. *)
-  (*     exists lw'. *)
-  (*     destruct H4; assert ((pc_a, pca_v) <> (a, v)) by congruence; simplify_map_eq; auto. *)
-  (* Qed. *)
+  Lemma incrementLPC_incrementPC_none regs :
+    incrementLPC regs = None <-> incrementPC (lreg_strip regs) = None.
+  Proof.
+    intros.
+    rewrite /incrementPC /incrementLPC.
+    rewrite /lreg_strip lookup_fmap; cbn.
+    destruct (regs !! PC) as [LX|] eqn:Heq ; rewrite Heq; cbn; last done.
+    destruct LX ; cbn ; [(clear; firstorder) | | (clear; firstorder)].
+    destruct sb as [? ? ? a' | ] ; eauto; cbn; last done.
+    destruct (a' + 1)%a eqn:Heq'; done.
+  Qed.
 
-  (* Lemma mem_implies_allow_load_map: *)
-  (*   ∀ (lregs : LReg)(lmem : LMem)(r2 : RegName) (pc_a : Addr) pca_v *)
-  (*     (lw lw' : LWord) p b e a v, *)
-  (*     (if ((a,v ) =? (pc_a, pca_v))%la *)
-  (*      then lmem = <[(pc_a, pca_v):=lw]> ∅ *)
-  (*      else lmem = <[(pc_a, pca_v):=lw]> (<[(a, v):=lw']> ∅)) *)
-  (*     → lregs !! r2 = Some (LCap p b e a v) *)
-  (*     → allow_load_map_or_true r2 lregs lmem. *)
-  (* Proof. *)
-  (*   intros lregs lmem r2 pc_a pca_v lw lw' p b e a v H4 Hrr2. *)
-  (*   destruct ((a,v) =? (pc_a, pca_v))%la eqn:Heq; cbn in Heq. *)
-  (*     + apply andb_true_iff in Heq. destruct Heq as [Heq1 Heq2]. *)
-  (*       apply Z.eqb_eq, finz_to_z_eq in Heq1. subst a. *)
-  (*       apply Nat.eqb_eq in Heq2. subst v. *)
-  (*       eapply mem_eq_implies_allow_load_map; eauto. *)
-  (*     + apply andb_false_iff in Heq. destruct Heq as [Heq | Heq] *)
-  (*     ; [ apply Z.eqb_neq in Heq |  apply Nat.eqb_neq in Heq ] *)
-  (*     ; eapply (mem_neq_implies_allow_load_map _ _ _ pc_a pca_v _ _ _ _ _ a v) ; eauto. *)
-  (*       left ; solve_addr. *)
-  (* Qed. *)
+  Lemma incrementLPC_fail_updatePC regs m etbl ecur:
+    incrementLPC regs = None ->
+    updatePC {| reg := (lreg_strip regs); mem := m; etable := etbl ; enumcur := ecur |} = None.
+  Proof.
+    intro Hincr. apply incrementLPC_incrementPC_none in Hincr.
+    by apply incrementPC_fail_updatePC.
+  Qed.
 
-  (* Lemma mem_implies_loadv: *)
-  (*   ∀ (pc_a : Addr) (pca_v : Version) (lw lw' : LWord) (a : Addr) *)
-  (*     (lmem : LMem) (loadv : LWord) v, *)
-  (*     (if ((a,v ) =? (pc_a, pca_v))%la *)
-  (*      then lmem = <[(pc_a, pca_v):=lw]> ∅ *)
-  (*      else lmem = <[(pc_a, pca_v):=lw]> (<[(a, v):=lw']> ∅))→ *)
-  (*     lmem !! (a,v) = Some loadv → *)
-  (*     loadv = (if ((a,v ) =? (pc_a, pca_v))%la then lw else lw'). *)
-  (* Proof. *)
-  (*   intros pc_a pca_v lw lw' a lmem loadv v H4 H6. *)
-  (*   destruct ((a,v ) =? (pc_a, pca_v))%la eqn:Heq; cbn in Heq ; rewrite H4 in H6. *)
-  (*   + apply andb_true_iff in Heq. destruct Heq as [Heq1 Heq2]. *)
-  (*     apply Z.eqb_eq, finz_to_z_eq in Heq1; subst a. *)
-  (*     apply Nat.eqb_eq in Heq2; subst v. *)
-  (*     by simplify_map_eq. *)
-  (*   + apply andb_false_iff in Heq. destruct Heq as [Heq | Heq] *)
-  (*     ; [ apply Z.eqb_neq in Heq |  apply Nat.eqb_neq in Heq ] *)
-  (*     ; rewrite lookup_insert_ne in H6; try congruence; try by simplify_map_eq. *)
-  (* Qed. *)
+
+  Lemma incrementLPC_success_updatePC regs m etbl ecur regs' :
+    incrementLPC regs = Some regs' ->
+    ∃ p b e a a' (v : Version),
+      regs !! PC = Some (LCap p b e a v) ∧
+      (a + 1)%a = Some a' ∧
+      updatePC {| reg := (lreg_strip regs); mem := m; etable := etbl ; enumcur := ecur |} =
+      Some (NextI,
+              {| reg := (<[PC:=WCap p b e a']> (lreg_strip regs));
+                mem := m;
+                etable := etbl ;
+                enumcur := ecur |})
+      ∧ regs' = <[ PC := (LCap p b e a' v) ]> regs.
+  Proof.
+    intro Hincr.
+    opose proof (incrementLPC_incrementPC_some _ _ Hincr) as HincrPC.
+    eapply (incrementPC_success_updatePC _ m etbl ecur) in HincrPC.
+    destruct HincrPC as (p'&b'&e'&a''&a'''&Hregs&Heq&Hupd&Hregseq).
+    rewrite /incrementLPC in Hincr.
+    destruct (regs !! PC) as [wpc |]; last done.
+    destruct_lword wpc; try done.
+    destruct (a + 1)%a as [a'|] eqn:Heq'; last done; simplify_eq.
+    rewrite /lreg_strip fmap_insert //= -/(lreg_strip regs)  in Hregseq.
+    exists p, b, e, a, a', v.
+    repeat (split; try done).
+    by rewrite Hupd Hregseq.
+  Qed.
 
   Definition exec_optL_Hash
     (lregs : LReg) (lmem : LMem)
@@ -164,6 +157,13 @@ Section cap_lang_rules.
         else None
     | _ => None
     end.
+
+  Lemma hash_lmemory_weaken lmem lm b e v :
+    Forall (λ a : Addr, ∃ lw, lmem !! (a, v) = Some lw) (finz.seq_between b e) ->
+    lmem ⊆ lm ->
+    (hash_lmemory_region lm b e v) =
+    (hash_lmemory_region lmem b e v).
+  Admitted.
 
   Lemma wp_hash Ep
     pc_p pc_b pc_e pc_a pc_v
@@ -183,82 +183,249 @@ Section cap_lang_rules.
             ([∗ map] la↦lw ∈ lmem, la ↦ₐ lw) ∗
             [∗ map] k↦y ∈ lregs', k ↦ᵣ y }}}.
   Proof.
-    iIntros (Hinstr Hvpc HPC Dregs Hmem_pc HaHash φ) "(>Hmem & >Hregs) Hφ".
-    rewrite -(insert_id lmem _ _ Hmem_pc).
-    iDestruct (big_sepM_insert_delete with "Hmem") as "[Hpc_a Hmem]"; cbn.
+    iIntros (Hinstr Hvpc HPC Dregs Hmem_pc HaHash φ) "(>Hmem & >Hmap) Hφ".
+    apply isCorrectLPC_isCorrectPC_iff in Hvpc; cbn in Hvpc.
+    iApply wp_lift_atomic_head_step_no_fork; auto.
+    iIntros (σ1 ns l1 l2 nt) "Hσ1 /=". destruct σ1; simpl.
+    iDestruct "Hσ1" as (lr lm vmap tbl_cur tbl_prev tbl_all)
+        "(Hr & Hm
+         & -> & Htbl_cur & Htbl_prev & Htbl_all
+         & HEC
+         & %Hdom_tbl1 & %Hdom_tbl2 & %Hdom_tbl3 & %Hdom_tbl4
+         & %HLinv)"
+    ; cbn in HLinv, Hdom_tbl1, Hdom_tbl2, Hdom_tbl3, Hdom_tbl4.
+    pose proof HLinv as HLinv'.
 
-    iApply (wp_instr_exec_opt Hvpc HPC Hinstr Dregs with "[$Hpc_a $Hregs Hmem Hφ]").
+    (* Derive necessary register values in r *)
+    iDestruct (gen_heap_valid_inclSepM with "Hr Hmap") as %Hregs.
+    have Hregs_pc := lookup_weaken _ _ _ _ HPC Hregs.
+    specialize (indom_lregs_incl _ _ _ Dregs Hregs) as Hri. unfold regs_of in Hri.
+    odestruct (Hri dst) as [ldstv [Hldst' Hldst] ]; first by set_solver+.
+    odestruct (Hri src) as [lsrcv [Hlsrc' Hlsrc] ]; first by set_solver+.
+
+    (* Derive necessary memory *)
+    iDestruct (gen_heap_valid_inclSepM with "Hm Hmem") as %Hmem.
+    iDestruct (gen_mem_valid_inSepM lmem lm with "Hm Hmem") as %Hma; eauto.
 
     iModIntro.
-    iIntros (σ) "(Hσ & Hregs &Hpc_a)".
-    iModIntro.
-    iIntros (wa) "(%Hppc & %Hpmema & %Hcorrpc & %Hdinstr) Hcred".
+    iSplitR.
+    by iPureIntro; apply normal_always_head_reducible.
+    iNext. iIntros (e2 σ2 efs Hpstep).
+    apply prim_step_exec_inv in Hpstep as (-> & -> & (c & -> & Hstep)).
+    iIntros "_".
+    iSplitR; auto; eapply step_exec_inv in Hstep; eauto.
+    2: rewrite -/((lword_get_word (LCap pc_p pc_b pc_e pc_a pc_v)))
+    ; eapply state_corresponds_reg_get_word ; eauto.
+    2: eapply state_corresponds_mem_correct_PC ; eauto; cbn ; eauto.
 
-    iApply (wp_wp2 (φ1 := exec_optL_Hash lregs lmem dst src)).
-    iApply wp_opt2_bind.
-    iApply wp_opt2_eqn.
+    set (srcv := lword_get_word lsrcv).
+    assert ( reg !! src = Some srcv ) as Hsrc
+        by (eapply state_corresponds_reg_get_word ; eauto).
+    rewrite /exec /= Hsrc /= in Hstep.
 
-    iDestruct (big_sepM_insert_delete _ _ _ lw with "[Hpc_a $Hmem]") as "Hmem"; iFrame.
-    rewrite insert_id; auto.
-    iMod (state_interp_transient_intro_nodfracs with "[$Hregs $Hσ $Hmem]") as "Hσ".
 
-    iApply (wp2_reg_lookup with "[$Hσ Hφ Hcred]") ; first by set_solver.
-    iIntros (lw2) "Hσ %Hlrs %Hrs".
+    (* src contains a capability *)
+    destruct (is_log_cap lsrcv) eqn:Hlsrcv; cycle 1; subst srcv; cbn in *.
+    { (* Fail : not a capability *)
+      destruct_lword lsrcv; cbn in * ; try congruence; clear Hlsrcv.
+      all: simplify_map_eq.
+      all: (iSplitR "Hφ Hmap Hmem"
+            ; [ iExists lr, lm, vmap,_,_,_; iFrame; auto
+              | iApply "Hφ" ; iFrame ; iFailCore Hash_fail_const
 
-    destruct (is_log_cap lw2) eqn:Hlw2; cycle 1.
+           ]).
+    }
+    destruct_lword lsrcv ; try (cbn in * ; congruence).
+    cbn in Hstep.
+
+
+    destruct (readAllowed p) eqn:HaRead; cycle 1; cbn in *.
     {
-      destruct_lword lw2 ; cbn in * ; simplify_eq.
-      all: iModIntro.
-      all: iDestruct (state_interp_transient_elim_abort with "Hσ") as "($ & Hregs & Hmem)".
-      all: rewrite big_sepM_fmap.
-      all: iApply ("Hφ" with "[$Hmem $Hregs]").
-      all: iPureIntro; constructor; by eapply Hash_fail_const.
+      simplify_map_eq.
+      iSplitR "Hφ Hmap Hmem"
+            ; [ iExists lr, lm, vmap,_,_,_; iFrame; auto
+              | iApply "Hφ" ; iFrame ; iFailCore Hash_fail_perm
+        ].
     }
 
-    destruct_lword lw2 ; cbn in * ; simplify_eq.
-    destruct (decide (readAllowed p = true)) as [Hread|Hread]
-    ; [|apply not_true_is_false in Hread] ; rewrite Hread ;cycle 1;cbn.
-    {
-      iModIntro.
-      iDestruct (state_interp_transient_elim_abort with "Hσ") as "($ & Hregs & Hmem)".
-      rewrite big_sepM_fmap.
-      iApply ("Hφ" with "[$Hmem $Hregs]").
-      iPureIntro; constructor; by eapply Hash_fail_perm.
+    set (lregs' := (<[ dst := LInt (hash_lmemory_region lm b e v) ]> lregs)).
+    set (lr' := (<[ dst := LInt (hash_lmemory_region lm b e v) ]> lr)).
+    assert (lreg_strip lregs' ⊆ lreg_strip lr') as Hlregs'_in_lr'.
+    { subst lregs' lr'.
+      by apply map_fmap_mono, insert_mono.
     }
 
-    pose proof (allow_hash_implies_hashv _ _ _ _ _ _ _ _ HaHash Hlrs Hread) as Hhash_mem.
 
-    rewrite updatePC_incrementPC.
-    iApply (wp_opt2_bind (k1 := fun x => Some x)).
-    iApply wp_opt2_eqn_both.
+    assert ( (lreg_strip lr') =
+               (<[ dst := WInt (hash_memory_region mem b e) ]> reg))
+      as Hstrip_lr'.
+    { subst lr'.
+      destruct HLinv as [ [Hstrips Hcurreg] _].
+      rewrite -Hstrips /lreg_strip !fmap_insert -/(lreg_strip lr) //=.
+      erewrite lmeasure_measure; eauto.
+    }
 
-    iDestruct (update_state_interp_transient_from_regs_mod (dst := dst) (lw2 := LInt (hash_lmemory_region lmem b e v)) with "Hσ") as "Hσ".
-    { set_solver. }
-    { by cbn. }
+    destruct (incrementLPC lregs') as  [?|] eqn:Hlregs'
+    ; pose proof Hlregs' as H'lregs'
+    ; cycle 1.
+    {
+      apply incrementLPC_fail_updatePC with (m:=mem) (etbl:=etable) (ecur:=enumcur) in Hlregs'.
+      eapply updatePC_fail_incl with
+        (regs' := lreg_strip lr') (m':=mem)
+        (etbl':=etable) (ecur':=enumcur) in Hlregs'
+      ; auto
+      ; cycle 1.
+      {
+        rewrite /lreg_strip lookup_fmap.
+        subst lregs' lr'.
+        apply fmap_is_Some.
+        destruct (decide (dst = PC)); simplify_map_eq ; auto.
+      }
+      rewrite Hstrip_lr' in Hlregs'.
+      match goal with
+      | Hstep :
+        match ?x with _ => _ end = (_,_) |- _ =>
+          replace x with (None : option Conf) in Hstep
+            by (destruct_lword lsrcv ; eauto)
+      end
+      ; simplify_eq.
+      subst lr'.
 
-    replace (WInt (hash_memory_region (mem σ) b e))
-      with ( lword_get_word  (LInt (hash_lmemory_region lmem b e v))).
-    2:{ cbn. admit. }
+      iSplitR "Hφ Hmap Hmem"
+      ; [ iExists lr, lm, vmap,_,_,_; iFrame; auto
+        | iApply "Hφ" ; iFrame].
+      eapply allow_hash_implies_hashv in HaHash; eauto.
+      subst lregs'.
+      rewrite {1}(hash_lmemory_weaken lmem lm) in H'lregs'; eauto.
+      cbn in *; iFailCore Hash_fail_invalid_PC.
+    }
+
+    (* PC has been incremented correctly *)
+    rewrite /update_reg /= in Hstep.
+    eapply (incrementLPC_success_updatePC _ mem etable enumcur) in Hlregs'
+        as (p1 & b1 & e1 & a1 & a_pc1 & v1 & HPC'' & Ha_pc' & HuPC & ->)
+    ; simplify_map_eq.
+    assert (dst <> PC) as Hdst by (subst lregs' ; intro ; simplify_map_eq).
+    eapply updatePC_success_incl with
+      (regs' := lreg_strip lr') (m':=mem) (etbl':=etable) (ecur':=enumcur) in HuPC
+    ; auto.
+    rewrite Hstrip_lr' in HuPC.
+    rewrite HuPC in Hstep; clear HuPC.
+    subst lregs' lr' ; simplify_eq ; simplify_map_eq.
+    eapply allow_hash_implies_hashv in HaHash; eauto.
 
 
-    iApply (wp2_opt_incrementPC with "[$Hσ Hcred Hφ]").
-    { now rewrite elem_of_dom (lookup_insert_dec HPC). }
-    iSplit; cbn; iIntros (φt' lrt') "Hσ %Heqn1 %Heqn2".
-    - iDestruct (state_interp_transient_elim_abort with "Hσ") as "($ & Hregs & Hmem)".
-      rewrite big_sepM_fmap.
-      iApply ("Hφ" with "[$Hmem $Hregs]").
-      iPureIntro.
-      eapply Hash_spec_failure.
-      by econstructor.
-    - iApply wp2_val.
-      cbn.
-      iMod (state_interp_transient_elim_commit with "Hσ") as "($ & Hregs & Hmem)".
-      rewrite big_sepM_fmap.
-      iApply ("Hφ" with "[$Hmem $Hregs]").
-      iPureIntro.
-      eapply Hash_spec_success; eauto.
-      split;eauto.
-  Admitted.
+    iMod ((gen_heap_update_inSepM _ _ dst (LInt (hash_lmemory_region lm b e v))) with "Hr Hmap")
+      as "[Hr Hmap]"; eauto.
+    iMod ((gen_heap_update_inSepM _ _ PC (LCap p1 b1 e1 a_pc1 v1)) with "Hr Hmap")
+      as "[Hr Hmap]"; eauto ; first by simplify_map_eq.
+
+    rewrite {1}(hash_lmemory_weaken lmem lm) in H'lregs'; eauto.
+
+
+    iFrame; iModIntro ; iSplitR "Hφ Hmap Hmem"
+    ; [| iApply "Hφ" ; iFrame; iPureIntro ; eapply Hash_spec_success; eauto]; cycle 1.
+    { split; eauto. }
+
+    iExists _, lm, vmap,_,_,_; iFrame; auto
+    ; iPureIntro; econstructor; eauto
+    ; repeat (split ; first done)
+    ; destruct HLinv as [ [Hstrips Hcur_reg] [Hdom Hroot] ]
+    ; cbn in *
+    ; last (split;eauto)
+    ; last done.
+    assert ( is_cur_word (LCap p1 b1 e1 a_pc1 v1) vmap ) as Hcur_PC.
+    { eapply lookup_weaken in HPC'' ; eauto.
+      eapply is_cur_lword_lea with (a' := a_pc1) ; cycle 2 ; eauto ; apply isWithin_refl.
+    }
+    erewrite lmeasure_measure; eauto.
+    eapply lreg_corresponds_insert_respects; eauto.
+    eapply lreg_corresponds_insert_respects; done.
+  Qed.
+
+  (* TODO old proof *)
+  (*   iIntros (Hinstr Hvpc HPC Dregs Hmem_pc HaHash φ) "(>Hmem & >Hregs) Hφ". *)
+  (*   rewrite -(insert_id lmem _ _ Hmem_pc). *)
+  (*   iDestruct (big_sepM_insert_delete with "Hmem") as "[Hpc_a Hmem]"; cbn. *)
+
+  (*   iApply (wp_instr_exec_opt Hvpc HPC Hinstr Dregs with "[$Hpc_a $Hregs Hmem Hφ]"). *)
+
+  (*   iModIntro. *)
+  (*   iIntros (σ) "(Hσ & Hregs &Hpc_a)". *)
+  (*   iModIntro. *)
+  (*   iIntros (wa) "(%Hppc & %Hpmema & %Hcorrpc & %Hdinstr) Hcred". *)
+
+  (*   iApply (wp_wp2 (φ1 := exec_optL_Hash lregs lmem dst src)). *)
+  (*   iApply wp_opt2_bind. *)
+  (*   iApply wp_opt2_eqn. *)
+
+  (*   iDestruct (big_sepM_insert_delete _ _ _ lw with "[Hpc_a $Hmem]") as "Hmem"; iFrame. *)
+  (*   rewrite insert_id; auto. *)
+  (*   iMod (state_interp_transient_intro_nodfracs with "[$Hregs $Hσ $Hmem]") as "Hσ". *)
+
+  (*   iApply (wp2_reg_lookup with "[$Hσ Hφ Hcred]") ; first by set_solver. *)
+  (*   iIntros (lw2) "Hσ %Hlrs %Hrs". *)
+
+  (*   destruct (is_log_cap lw2) eqn:Hlw2; cycle 1. *)
+  (*   { *)
+  (*     destruct_lword lw2 ; cbn in * ; simplify_eq. *)
+  (*     all: iModIntro. *)
+  (*     all: iDestruct (state_interp_transient_elim_abort with "Hσ") as "($ & Hregs & Hmem)". *)
+  (*     all: rewrite big_sepM_fmap. *)
+  (*     all: iApply ("Hφ" with "[$Hmem $Hregs]"). *)
+  (*     all: iPureIntro; constructor; by eapply Hash_fail_const. *)
+  (*   } *)
+
+  (*   destruct_lword lw2 ; cbn in * ; simplify_eq. *)
+  (*   destruct (decide (readAllowed p = true)) as [Hread|Hread] *)
+  (*   ; [|apply not_true_is_false in Hread] ; rewrite Hread ;cycle 1;cbn. *)
+  (*   { *)
+  (*     iModIntro. *)
+  (*     iDestruct (state_interp_transient_elim_abort with "Hσ") as "($ & Hregs & Hmem)". *)
+  (*     rewrite big_sepM_fmap. *)
+  (*     iApply ("Hφ" with "[$Hmem $Hregs]"). *)
+  (*     iPureIntro; constructor; by eapply Hash_fail_perm. *)
+  (*   } *)
+
+  (*   pose proof (allow_hash_implies_hashv _ _ _ _ _ _ _ _ HaHash Hlrs Hread) as Hhash_mem. *)
+
+  (*   rewrite updatePC_incrementPC. *)
+  (*   iApply (wp_opt2_bind (k1 := fun x => Some x)). *)
+  (*   iApply wp_opt2_eqn_both. *)
+
+  (*   iDestruct (update_state_interp_transient_from_regs_mod (dst := dst) (lw2 := LInt (hash_lmemory_region lmem b e v)) with "Hσ") as "Hσ". *)
+  (*   { set_solver. } *)
+  (*   { by cbn. } *)
+
+  (*   replace (WInt (hash_memory_region (mem σ) b e)) *)
+  (*     with ( lword_get_word  (LInt (hash_lmemory_region lmem b e v))). *)
+  (*   2:{ cbn. admit. } *)
+
+
+  (*   iApply (wp2_opt_incrementPC with "[$Hσ Hcred Hφ]"). *)
+  (*   { now rewrite elem_of_dom (lookup_insert_dec HPC). } *)
+  (*   iSplit; cbn; iIntros (φt' lrt') "Hσ %Heqn1 %Heqn2". *)
+  (*   - iDestruct (state_interp_transient_elim_abort with "Hσ") as "($ & Hregs & Hmem)". *)
+  (*     rewrite big_sepM_fmap. *)
+  (*     iApply ("Hφ" with "[$Hmem $Hregs]"). *)
+  (*     iPureIntro. *)
+  (*     eapply Hash_spec_failure. *)
+  (*     by econstructor. *)
+  (*   - iApply wp2_val. *)
+  (*     cbn. *)
+  (*     iMod (state_interp_transient_elim_commit with "Hσ") as "($ & Hregs & Hmem)". *)
+  (*     rewrite big_sepM_fmap. *)
+  (*     iApply ("Hφ" with "[$Hmem $Hregs]"). *)
+  (*     iPureIntro. *)
+  (*     eapply Hash_spec_success; eauto. *)
+  (*     split;eauto. *)
+  (* Admitted. *)
+
+(* Global Instance laddr_eqdec: EqDecision LAddr. *)
+(* Proof. apply _. Defined. *)
+(* Global Instance laddr_countable: Countable LAddr. *)
+(* Admitted. *)
+
 
   Lemma wp_hash_success Ep
     pc_p pc_b pc_e pc_a pc_a' pc_v
@@ -270,6 +437,8 @@ Section cap_lang_rules.
     isCorrectLPC (LCap pc_p pc_b pc_e pc_a pc_v) →
     readAllowed p = true →
     (pc_a + 1)%a = Some pc_a' →
+    pc_a ∉ finz.seq_between b e ->
+    length ws = finz.dist b e ->
 
     {{{ ▷ PC ↦ᵣ LCap pc_p pc_b pc_e pc_a pc_v
         ∗ ▷ (pc_a, pc_v) ↦ₐ lw
@@ -281,26 +450,28 @@ Section cap_lang_rules.
       {{{ RET NextIV;
           PC ↦ᵣ LCap pc_p pc_b pc_e pc_a' pc_v
           ∗ (pc_a, pc_v) ↦ₐ lw
-          ∗ dst ↦ᵣ LWInt (hash ws)
+          ∗ dst ↦ᵣ LWInt (hash (lword_get_word <$> ws))
           ∗ src ↦ᵣ LCap p b e a v
           ∗ [[ b , e ]] ↦ₐ{ v } [[ ws ]]
       }}}.
   Proof.
-    intros Hdecode HcorrectPC Hread_allowed Hpca'.
+    intros Hdecode HcorrectPC Hread_allowed Hpca' Hpca_ne Hlen_ws.
     iIntros (φ) "(>HPC & >Hpca & >Hdst & >Hsrc & >Hmem) Hφ".
     iDestruct (map_of_regs_3 with "HPC Hdst Hsrc") as "[Hmap (%&%&%)]".
     rewrite /region_mapsto.
     iDestruct ( big_sepL2_to_big_sepM with "Hmem") as "Hmem".
-    { admit. }
+    { apply NoDup_fmap_2.
+      - intros a1 a2 Haeq; congruence.
+      - by apply finz_seq_between_NoDup.
+    }
     iDestruct (big_sepM_insert with "[$Hmem $Hpca]") as "Hmem".
-    { admit. }
+    { shelve. }
 
     iApply (wp_hash with "[$]"); eauto.
     { by simplify_map_eq. }
     { by rewrite !dom_insert; set_solver+. }
     { by simplify_map_eq. }
     {
-
       rewrite /allow_hash_map_or_true.
       exists p,b,e,a,v.
       split.
@@ -311,19 +482,92 @@ Section cap_lang_rules.
       - match goal with
         | H: _ |- context [decide ?x] => destruct (decide x)
         end; last done.
-        (* rewrite /reg_allows_hash in r; destruct r as [r _]. *)
-        (* rewrite lookup_insert_ne // in r. *)
-        (* rewrite lookup_insert_ne // in r. *)
-        (* rewri *)
         apply Forall_forall.
         intros a' Ha'.
-        admit.
-        (* rewrite //. *)
-
+        destruct (decide (a' = pc_a)); simplify_map_eq.
+        rewrite lookup_insert_ne; last congruence.
+        rewrite -/(is_Some (_ !! (a',v))).
+        apply elem_of_dom.
+        rewrite dom_list_to_map_L.
+        apply elem_of_list_to_set.
+        rewrite fst_zip.
+        2: { by rewrite Hlen_ws map_length finz_seq_between_length. }
+        apply elem_of_list_fmap.
+        eexists ; split; done.
     }
+    iNext. iIntros (lregs' retv) "(%Hspec & Hmem & Hregs)".
+    destruct Hspec; cycle 1.
+    { destruct X; simplify_map_eq; try congruence.
+      incrementLPC_inv; simplify_map_eq; eauto; congruence.
+    }
+    iApply "Hφ".
+    incrementLPC_inv; simplify_map_eq; eauto.
+    rewrite (insert_commute _ PC dst) // insert_insert.
+    rewrite (insert_commute _ dst PC) // insert_insert.
+    iDestruct (regs_of_map_3 with "Hregs") as "(?&?&?)"; eauto; iFrame.
+
+    replace
+      (hash_lmemory_region (<[(x2, x3):=lw]> (list_to_map (zip (map (λ a1 : Addr, (a1, v)) (finz.seq_between b e)) ws))) b0 e0 v0)
+      with (hash (lword_get_word <$> ws)).
+    2: {
+      rewrite /hash_lmemory_region.
+      f_equal.
+      f_equal.
+      destruct H2 as [? _]; simplify_map_eq.
+      rewrite map_filter_insert_not; cycle 1.
+      { intros w' [ ? ? ]; cbn in *; simplify_eq. }
 
 
+      Set Nested Proofs Allowed.
+  Lemma map_filter_alt':
+    ∀ {K : Type} {M : Type → Type} {H : FMap M} {H0 : ∀ A : Type, Lookup K A (M A)} {H1 : ∀ A : Type, Empty (M A)}
+      {H2 : ∀ A : Type, PartialAlter K A (M A)} {H3 : OMap M} {H4 : Merge M} {H5 : ∀ A : Type, MapFold K A (M A)}
+      {EqDecision0 : EqDecision K},
+      FinMap K M
+    → ∀ {A : Type} (P : K * A → Prop) {H7 : ∀ x : K * A, Decision (P x)}
+        (l : list (K * A)),
+        NoDup l ->
+        filter P l = map_to_list (filter P (list_to_map l)).
+    Proof.
+      intros * ? * Hnodup.
+      induction l; cbn.
+      - by rewrite map_filter_empty map_to_list_empty.
+      - apply NoDup_cons in Hnodup. destruct Hnodup as [Hal Hnodup].
+        destruct a as [a1 a2].
+        destruct (decide (P (a1,a2))); rewrite IHl; auto.
+        + rewrite map_filter_insert_True; last done.
+          admit.
+        + rewrite map_filter_insert_False; last done.
+          admit.
+    Admitted.
+    admit.
+    (* rewrite map_filter_alt'. *)
+    }
+    iFrame.
+    iDestruct (big_sepM_insert with "Hmem") as "[Ha Hmem]".
+    { apply not_elem_of_list_to_map.
+      rewrite fst_zip.
+      2: { by rewrite Hlen_ws map_length finz_seq_between_length. }
+      intro Hcontra.
+      apply elem_of_list_fmap in Hcontra.
+      destruct Hcontra as [? [? ?] ]; simplify_eq.
+    }
+    iFrame.
+    iDestruct ( big_sepM_to_big_sepL2 with "Hmem") as "Hmem".
+    { apply NoDup_fmap_2.
+      - intros a1 a2 Haeq; congruence.
+      - by apply finz_seq_between_NoDup.
+    }
+    { by rewrite Hlen_ws map_length finz_seq_between_length. }
+    iFrame.
 
+    Unshelve.
+    {
+      apply not_elem_of_list_to_map_1.
+      intro Hcontra.
+      eapply fst_elem_of_cons, elem_of_list_fmap in Hcontra.
+      destruct Hcontra as [? [? ?] ]; simplify_eq.
+    }
   Admitted.
 
   Lemma wp_hash_success_same Ep
@@ -345,7 +589,7 @@ Section cap_lang_rules.
       {{{ RET NextIV;
           PC ↦ᵣ LCap pc_p pc_b pc_e pc_a' pc_v
           ∗ (pc_a, pc_v) ↦ₐ lw
-          ∗ dst ↦ᵣ LWInt (hash ws)
+          ∗ dst ↦ᵣ LWInt (hash (lword_get_word <$> ws))
           ∗ [[ b , e ]] ↦ₐ{ v } [[ ws ]]
       }}}.
   Proof.
@@ -372,7 +616,7 @@ Section cap_lang_rules.
       Instr Executable @ Ep
       {{{ RET NextIV;
           PC ↦ᵣ LCap pc_p pc_b pc_e pc_a' pc_v
-          ∗ dst ↦ᵣ LWInt (hash (ws++[lw]++ws'))
+          ∗ dst ↦ᵣ LWInt (hash (lword_get_word <$> (ws++[lw]++ws')))
           ∗ src ↦ᵣ LCap p b e a v
           ∗ [[ b , pc_a ]] ↦ₐ{ v } [[ ws ]]
           ∗ (pc_a, pc_v) ↦ₐ lw
